Generalize some timing automation

timing/examples/FreeRTOS_tasks_noasserts_proofs_clz.v
@@ -3,100 +3,64 @@ Require Import riscvTiming.
 Import RISCVNotations.
 Require Import memsolve.
 
-Definition start_vTaskSwitchContext : N := 0x8000137c.
-Definition end_vTaskSwitchContext : N := 0x8000144c.
-
+(* Some machinery describing the CPU *)
 Variable ML : N.
 Variable ML_pos : 1 <= ML.
-
 Module riscv_toa.
     Definition time_of_addr (s : store) (a : addr) : N :=
         match neorv32_cycles_upper_bound ML s (RTOSDemo_NoAsserts_Clz a) with
-        | Some x => x | _ => 0 end.
+        | Some x => x | _ => 999 end.
 End riscv_toa.
-
 Module riscvT := MakeTimingContents riscvTiming riscv_toa.
 Export riscvT.
-
 Definition cycle_count_of_trace := cycle_count_of_trace time_of_addr.
 
+(* These expressions pop up a lot and I don't like seeing them, so just fold them up
+   - time_mem    = The time in clock cycles of a memory access
+   - time_branch = The time in clock cycles of a successful/taken branch
+*)
 Definition time_mem : N :=
     5 + (ML - 2).
-
 Definition time_branch : N :=
     5 + (ML - 1).
 
+(* The doubleword in static memory (offset of gp) that determines if the scheduler
+   is suspended. The scheduler should be suspended when any critical behavior
+   is ongoing that could be disrupted by context switching
+   - Memory allocation
+   - Atomic operations
+   - Modifying shared memory
+   - Performance optimization
+*)
 Definition uxSchedulerSuspended (gp : N) (mem : addr -> N) : N :=
-    (* mem Ⓓ[2144 + gp]. *)
-    (* This should actually be the below expression. Unclear on whether lifter
-       has bug, seems like it isn't treating immediate as signed
-    *)
     mem Ⓓ[gp ⊖ 1952].
 
-Definition addr_xYieldPendings (gp : N) : N :=
+(* The address of the doubleword in static memory that is nonzero when a task is
+   ready to "yield," or signal that a context switch needs to occur (either 
+   voluntarily or involuntarily)
+*)
+Definition addr_xYieldPendings (gp : N) : addr :=
     gp - 1932.
 
+(* A pointer in static memory to the Current Task Control Block (TCB). The TCB
+   is a data structure containing all essential information for managing a task.
+*)
 Definition pxCurrentTCB (gp : N) (mem : addr -> N) : N :=
-    (* mem Ⓓ[2200 + gp]. *)
-    (* Same as above *)
     mem Ⓓ[gp ⊖ 1896].
 
+(* The doubleword in static memory that records the highest priority out of all
+   currently-ready tasks.
+*)
 Definition uxTopReadyPriority (gp : N) (mem : addr -> N) : N :=
     mem Ⓓ[gp ⊖ 1920].
 
-Definition addr_pxReadyTasksLists (gp : N) : N :=
+(* The address in static memory of a list of linked-lists that record all currently-
+   ready tasks. The index into pxReadyTasksLists indicates those tasks' priority.
+*)
+Definition addr_pxReadyTasksLists (gp : N) : addr :=
     gp ⊖ 924.
 
-Definition vTaskSwitchContext_exit (t:trace) :=
-  match t with (Addr a,_)::_ => match a with
-  | 0x8000138c | 0x8000144c => true
-  | _ => false
-  end | _ => false end.
-
-(* TODO : Rewrite postconditions, the if conditions are garbage from earlier versions *)
-Definition timing_postcondition (t : trace) (gp : N) (mem : addr -> N) : Prop :=
-    if (uxSchedulerSuspended gp mem) =? 0 then
-        cycle_count_of_trace t = 25 + 3 * time_branch + 17 * time_mem
-        + (if (mem Ⓓ[(gp ⊖ 920) ⊕ ((31 ⊖ (clz (uxTopReadyPriority gp mem) 32)) * 20)])
-            =? ((gp ⊖ 916) ⊕ (31 ⊖ clz (uxTopReadyPriority gp mem) 32) * 20)
-            then 22 + clz (mem Ⓓ[ 4294965376 + gp ]) 32 + 5 * time_mem else
-            19 + time_branch + clz (mem Ⓓ[ 4294965376 + gp ]) 32 + 3 * time_mem
-        )
-    else
-        cycle_count_of_trace t = 5 + time_branch + 2 * time_mem.
-
-Definition __global_pointer : N := 0x80080800.
-Definition __global_size : N := 2048.
-Definition __stack_pointer : N :=
-    (* Section 4.4.2. RAM Layout - 
-        The stack starts at the very end of the RAM at address ORIGIN(ram) + LENGTH(ram) - 4.
-        The stack grows downwards.*)
-    (* https://cdn.hackaday.io/files/1741677451560928/NEORV32.pdf *)
-    (2 ^ 32) - 4.
-
-Definition vTaskSwitchContext_stack_frame_size : N := 16.
-
-Definition gp_sp_noverlap (gp sp : N) : Prop :=
-    ~overlap 32 (gp ⊖ __global_size) __global_size (sp ⊖ vTaskSwitchContext_stack_frame_size) vTaskSwitchContext_stack_frame_size.
-
-Fixpoint subtrace_since_address (t : trace) (a : addr) : trace :=
-    match t with
-    | (Addr a', st) :: tl => if (a =? a') then (Addr a', st) :: nil else
-        (Addr a', st) :: subtrace_since_address tl a
-    | _ => nil
-    end.
-
-Fixpoint subtrace_before_address (t : trace) (a : addr) : trace :=
-    match t with
-    | (Addr a', st) :: tl => if (a =? a') then tl else
-        subtrace_before_address tl a
-    | _ => nil
-    end.
-
-Definition time_before_address (t : trace) (a : addr) :=
-    cycle_count_of_trace (subtrace_before_address t a).
-
-(* The goal with the above function is to use for function timing invariants, e.g.
+(* The goal with the below functions is to use for function timing invariants, e.g.
         cycle_count_of_trace t' = 
             func_time + cycle_count_of_trace (subtrace_before_address t' func_entry_addr))
     This would be nice because then you don't have to worry about annoying arithmetic.
@@ -117,6 +81,39 @@ Definition time_before_address (t : trace) (a : addr) :=
     Will have to revisit later, definitely need something like this for scaling up.
 *)
 
+Fixpoint subtrace_since_address (t : trace) (a : addr) : trace :=
+    match t with
+    | (Addr a', st) :: tl => if (a =? a') then (Addr a', st) :: nil else
+        (Addr a', st) :: subtrace_since_address tl a
+    | _ => nil
+    end.
+
+Fixpoint subtrace_before_address (t : trace) (a : addr) : trace :=
+    match t with
+    | (Addr a', st) :: tl => if (a =? a') then tl else
+        subtrace_before_address tl a
+    | _ => nil
+    end.
+
+Definition time_before_address (t : trace) (a : addr) : N :=
+    cycle_count_of_trace (subtrace_before_address t a).
+
+(* The size of static memory (at the bottom of memory) and stack memory (at the
+   top)
+*)
+Definition __global_size : N := 2048.
+Definition vTaskSwitchContext_stack_frame_size : N := 16.
+
+(* What follows are a list of assumptions we make about the well-formedness of
+   static and stack memory. For example: static and stack memory should not overlap
+   (this would be a stack overflow)
+*)
+Definition gp_sp_noverlap (gp sp : N) : Prop :=
+    ~overlap 32 (gp ⊖ __global_size) __global_size (sp ⊖ vTaskSwitchContext_stack_frame_size) vTaskSwitchContext_stack_frame_size.
+
+(* These two definitions state that any two of the above buffers we're interested
+   in do not overlap
+*)
 Definition static_buffer_lengths_in_bytes (a : addr) : option N :=
     match a with
     (* uxSchedulerSuspended *)
@@ -127,7 +124,6 @@ Definition static_buffer_lengths_in_bytes (a : addr) : option N :=
     | 1896 
     (* uxTopReadyPriority *)
     | 1920 => Some 4
-    (* TODO : Prove that smem_well_formed doesn't break with this in it *)
     | _ => None
     end.
 
@@ -140,42 +136,93 @@ Definition smem_well_formed (gp : N) : Prop :=
                 (gp ⊖ x) len_x
                 (gp ⊖ y) len_y.
 
-Definition pxCurrentTCB_noverlap_clz_static (gp : N) mem : Prop :=
+(* I don't yet know the significance of the address
+      gp ⊖ 920 ⊕ (31 ⊖ clz (uxTopReadyPriority gp mem) 32) * 20
+   but it appears very frequently and it must not overlap with things like the
+   TCB or stack memory. Some of these assumptions can actually be proven due to 
+   the boundaries of clz (count leading zeroes) being 0..32
+*)
+Definition pxCurrentTCB_noverlap_clz_static (gp : N) (mem : addr -> N) : Prop :=
     ~ overlap 32
         (48 + pxCurrentTCB gp mem) 4
-        (gp ⊖ 920 ⊕ (31 ⊖ clz (mem Ⓓ[ gp ⊖ 1920 ]) 32) * 20) 4.
+        (gp ⊖ 920 ⊕ (31 ⊖ clz (uxTopReadyPriority gp mem) 32) * 20) 4.
 
 Definition clz_noverlap_smem (gp : N) mem : Prop :=
     forall x len_x,
         static_buffer_lengths_in_bytes x = Some len_x ->
         ~ overlap 32
             (gp ⊖ x) len_x
-            (gp ⊖ 920 ⊕ (31 ⊖ clz (mem Ⓓ[ gp ⊖ 1920 ]) 32) * 20) 4.
+            (gp ⊖ 920 ⊕ (31 ⊖ clz (uxTopReadyPriority gp mem) 32) * 20) 4.
 
-Definition pxCurrentTCB_noverlap_static (gp : N) mem : Prop :=
+(* The TCB doesn't overlap static memory or the stack frame *)
+Definition pxCurrentTCB_noverlap_static (gp : N) (mem : addr -> N) : Prop :=
     forall x len_x,
         static_buffer_lengths_in_bytes x = Some len_x ->
         ~ overlap 32
             (48 + pxCurrentTCB gp mem) 4
             (gp ⊖ x) len_x.
 
-Definition pxCurrentTCB_noverlap_stackframe (gp base_sp : N) mem : Prop :=
+Definition pxCurrentTCB_noverlap_stackframe (gp base_sp : N) (mem : addr -> N) : Prop :=
     ~ overlap 32
         (48 + pxCurrentTCB gp mem) 4
         (base_sp ⊖ 16) 16.
 
-Definition mem_pxCurrentTCB_noverlap_stackframe (gp base_sp : N) mem : Prop :=
+(* The address contained in the current TCB doesn't overlap with static memory
+   or the stack frame *)
+Definition mem_pxCurrentTCB_noverlap_stackframe (gp base_sp : N) (mem : addr -> N) : Prop :=
     ~ overlap 32
         (mem Ⓓ[48 + pxCurrentTCB gp mem]) 4
         (base_sp ⊖ 16) 16.
 
-Definition mem_pxCurrentTCB_noverlap_static (gp : N) mem : Prop :=
+Definition mem_pxCurrentTCB_noverlap_static (gp : N) (mem : addr -> N) : Prop :=
     forall x len_x,
         static_buffer_lengths_in_bytes x = Some len_x ->
         ~ overlap 32
             (mem Ⓓ[48 + pxCurrentTCB gp mem]) 4
             (gp ⊖ x) len_x.
 
+(* Offsets into the address contained in the current TCB don't overlap with 
+   the clz address or stack memory *)
+Definition offset_mem_pxCurrentTCB_noverlap_clz (gp : N) (mem : addr -> N) : Prop :=
+    forall k, k = 8 \/ k = 12 ->
+        ~ overlap 32
+            (k + mem Ⓓ[48 + pxCurrentTCB gp mem]) 4
+            (gp ⊖ 920 ⊕ (31 ⊖ clz (uxTopReadyPriority gp mem) 32) * 20) 4.
+
+Definition clz_noverlap_sframe (gp base_sp : N) (mem : addr -> N) : Prop :=
+    ~ overlap 32 
+        (base_sp ⊖ 16) 16
+        (gp ⊖ 920 ⊕ (31 ⊖ clz (uxTopReadyPriority gp mem) 32) * 20) 4.
+
+(* An offset into the buffer at the clz address doesn't overlap with static
+   memory or the stack frame *)
+Definition mem4_pxCurrentTCB_noverlap_stackframe (gp base_sp : N) (mem : addr -> N) : Prop :=
+        ~ overlap 32
+        (base_sp ⊖ 16) 16
+            (4 + mem Ⓓ[gp ⊖ 920 ⊕ (31 ⊖ clz (uxTopReadyPriority gp mem) 32) * 20]) 4.
+
+Definition mem4_pxCurrentTCB_noverlap_static (gp : N) (mem : addr -> N) : Prop :=
+    forall x len_x,
+        static_buffer_lengths_in_bytes x = Some len_x ->
+        ~ overlap 32
+            (gp ⊖ x) 4
+            (4 + mem Ⓓ[gp ⊖ 920 ⊕ (31 ⊖ clz (uxTopReadyPriority gp mem) 32) * 20]) 4.
+
+(* An offset into the buffer at an offset into the buffer at the clz address 
+   doesn't overlap with static memory or the stack frame *)
+Definition mem4_mem4_noverlap_stackframe (gp base_sp : N) (mem : addr -> N) :=
+    ~ overlap 32
+        (base_sp ⊖ 16) 16
+        (4 + mem Ⓓ[ 4 + mem Ⓓ[ gp ⊖ 920 ⊕ (31 ⊖ clz (uxTopReadyPriority gp mem) 32) * 20 ] ]) 4.
+
+Definition mem4_mem4_noverlap_static (gp : N) (mem : addr -> N) :=
+    forall x len_x,
+        static_buffer_lengths_in_bytes x = Some len_x ->
+        ~ overlap 32
+            (gp ⊖ x) 4
+            (4 + mem Ⓓ[ 4 + mem Ⓓ[ gp ⊖ 920 ⊕ (31 ⊖ clz (uxTopReadyPriority gp mem) 32) * 20 ] ]) 4.
+
+(* Stick them all together *)
 Definition common_noverlaps gp base_sp mem : Prop :=
     gp_sp_noverlap gp base_sp /\
     smem_well_formed gp /\
@@ -184,9 +231,37 @@ Definition common_noverlaps gp base_sp mem : Prop :=
     pxCurrentTCB_noverlap_clz_static gp mem /\
     clz_noverlap_smem gp mem /\
     mem_pxCurrentTCB_noverlap_stackframe gp base_sp mem /\
-    mem_pxCurrentTCB_noverlap_static gp mem.
+    mem_pxCurrentTCB_noverlap_static gp mem /\
+    offset_mem_pxCurrentTCB_noverlap_clz gp mem /\
+    clz_noverlap_sframe gp base_sp mem /\
+    mem4_pxCurrentTCB_noverlap_stackframe gp base_sp mem /\
+    mem4_pxCurrentTCB_noverlap_static gp mem.
 
-Definition vTaskSwitchContext_timing_invs (_ : store) (p : addr) (base_sp : N) (t:trace) :=
+Definition time_of_vTaskSwitchContext (t : trace) (gp : N) (mem : addr -> N) : Prop :=
+    (* is the scheduler suspended *)
+    if (uxSchedulerSuspended gp mem) =? 0 then
+        cycle_count_of_trace t = (* total number of cycles equals... *)
+        25 + 3 * time_branch + 17 * time_mem
+            (* This branch condition isn't well-documented, need to dig into source *)
+          + (if (mem Ⓓ[ 4 + mem Ⓓ[ gp ⊖ 920 ⊕ (31 ⊖ clz (uxTopReadyPriority gp mem) 32) * 20 ] ])
+              =? ((gp ⊖ 916) ⊕ (31 ⊖ clz (uxTopReadyPriority gp mem) 32) * 20)
+              then 
+                22 + (clz (uxTopReadyPriority gp mem) 32) + 5 * time_mem 
+              else
+                19 + time_branch + (clz (uxTopReadyPriority gp mem) 32) + 3 * time_mem
+              (* time_branch = 5 + (memory latency - 1), # of cycles for a successful/taken branch *)
+              (* time_mem = 5 + (memory latency - 2), # of cycles for a memory retreival *)
+          )
+    else
+        cycle_count_of_trace t = 5 + time_branch + 2 * time_mem.
+
+(* The invariant set for the proof. These are waypoints that guide us towards 
+   the postcondition. We state properties here that we want to remember for later
+   in the proof (anything not in an invariant is forgotten after a branch).
+   The properties that we state help us prove the postcondition. We must prove
+   each invariant throughout the proof. *)
+Definition vTaskSwitchContext_timing_invs (_ : store) (p : addr) 
+    (base_sp gp : N) (base_mem : addr -> N) (t:trace) : option Prop :=
 match t with (Addr a, s) :: t' => match a with
     (* vApplicationStackOverflowHook *)
     (* NOTE : This function intentionally goes into an infinite loop when a
@@ -196,660 +271,364 @@ match t with (Addr a, s) :: t' => match a with
     | 0x8000e804 => Some True
     (* vTaskSwitchContext *)
     | 0x80001380 => Some (
-        exists mem gp, s V_MEM32 = Ⓜmem /\ s R_GP = Ⓓgp /\ s R_SP = Ⓓbase_sp 
-            /\ s R_A4 = Ⓓ(uxSchedulerSuspended gp mem) /\
+        exists mem, s V_MEM32 = Ⓜmem /\ s R_GP = Ⓓgp /\ s R_SP = Ⓓbase_sp 
+            /\ s R_A4 = Ⓓ(uxSchedulerSuspended gp base_mem) /\
             common_noverlaps gp base_sp mem /\
+            mem4_mem4_noverlap_stackframe gp base_sp mem /\
+            mem4_mem4_noverlap_static gp mem /\
+            ~ overlap 32
+                (gp ⊖ 920 ⊕ (31 ⊖ clz (uxTopReadyPriority gp mem) 32) * 20) 4
+                (4 + mem Ⓓ[ gp ⊖ 920 ⊕ (31 ⊖ clz (uxTopReadyPriority gp mem) 32) * 20 ] ) 4 /\
+            ~ overlap 32
+                (gp ⊖ 920 ⊕ (31 ⊖ clz (uxTopReadyPriority gp mem) 32) * 20) 4
+                (mem Ⓓ[4 + mem Ⓓ[ gp ⊖ 920 ⊕ (31 ⊖ clz (uxTopReadyPriority gp mem) 32) * 20 ]]) 4 /\
+            uxTopReadyPriority gp mem = uxTopReadyPriority gp base_mem /\
+            mem Ⓓ[ 4 + mem Ⓓ[ gp ⊖ 920 + (31 ⊖ clz (uxTopReadyPriority gp mem) 32) * 20 ] ] =
+            base_mem Ⓓ[ 4 + base_mem Ⓓ[ gp ⊖ 920 + (31 ⊖ clz (uxTopReadyPriority gp base_mem) 32) * 20 ] ]  /\
         cycle_count_of_trace t' = time_mem)
-    | 0x800013b4 => Some (exists mem gp, s V_MEM32 = Ⓜmem /\ 
-        s R_GP = Ⓓgp /\ s R_SP = Ⓓ(base_sp ⊖ 16) /\
-        s R_A5 = Ⓓ(mem Ⓓ[48 + pxCurrentTCB gp mem]) /\
-        s R_A2 = Ⓓ(mem Ⓓ[mem Ⓓ[48 + pxCurrentTCB gp mem]]) /\
-        s R_A4 = Ⓓ((0xa5a5a << 12) + 1445) /\
+    | 0x800013b4 => Some (exists mem, s V_MEM32 = Ⓜmem /\ 
+        s R_GP = Ⓓgp /\
         common_noverlaps gp base_sp mem /\
-        (uxSchedulerSuspended gp mem =? 0) = true /\
+        mem4_mem4_noverlap_stackframe gp base_sp mem /\
+        mem4_mem4_noverlap_static gp mem /\
+        ~ overlap 32
+            (gp ⊖ 920 ⊕ (31 ⊖ clz (uxTopReadyPriority gp mem) 32) * 20) 4
+            (4 + mem Ⓓ[ gp ⊖ 920 ⊕ (31 ⊖ clz (uxTopReadyPriority gp mem) 32) * 20 ] ) 4 /\
+        ~ overlap 32
+            (gp ⊖ 920 ⊕ (31 ⊖ clz (uxTopReadyPriority gp mem) 32) * 20) 4
+            (mem Ⓓ[4 + mem Ⓓ[ gp ⊖ 920 ⊕ (31 ⊖ clz (uxTopReadyPriority gp mem) 32) * 20 ]]) 4 /\
+        uxTopReadyPriority gp mem = uxTopReadyPriority gp base_mem /\
+        mem Ⓓ[ 4 + mem Ⓓ[ gp ⊖ 920 + (31 ⊖ clz (uxTopReadyPriority gp mem) 32) * 20 ] ] =
+            base_mem Ⓓ[ 4 + base_mem Ⓓ[ gp ⊖ 920 + (31 ⊖ clz (uxTopReadyPriority gp base_mem) 32) * 20 ] ]  /\
+        (uxSchedulerSuspended gp base_mem =? 0) = true /\
         cycle_count_of_trace t' = 6 + 7 * time_mem + time_branch)
-    | 0x800013bc => Some (exists mem gp, s V_MEM32 = Ⓜmem /\ 
-        s R_GP = Ⓓgp /\ s R_SP = Ⓓ(base_sp ⊖ 16) /\
-        s R_A2 = Ⓓ(mem Ⓓ[mem Ⓓ[48 + pxCurrentTCB gp mem]]) /\
-        s R_A3 = Ⓓ(mem Ⓓ[4 + mem Ⓓ[48 + pxCurrentTCB gp mem]]) /\
-        s R_A5 = Ⓓ(mem Ⓓ[48 + pxCurrentTCB gp mem]) /\
+    | 0x800013bc => Some (exists mem, s V_MEM32 = Ⓜmem /\ 
+        s R_GP = Ⓓgp /\
         common_noverlaps gp base_sp mem /\
-        (uxSchedulerSuspended gp mem =? 0) = true /\
-        (mem Ⓓ[ mem Ⓓ[ 48 + pxCurrentTCB gp mem ] ] =? 0xa5a5a5a5) = true /\
+        mem4_mem4_noverlap_stackframe gp base_sp mem /\
+        mem4_mem4_noverlap_static gp mem /\
+        ~ overlap 32
+            (gp ⊖ 920 ⊕ (31 ⊖ clz (uxTopReadyPriority gp mem) 32) * 20) 4
+            (4 + mem Ⓓ[ gp ⊖ 920 ⊕ (31 ⊖ clz (uxTopReadyPriority gp mem) 32) * 20 ] ) 4 /\
+        ~ overlap 32
+            (gp ⊖ 920 ⊕ (31 ⊖ clz (uxTopReadyPriority gp mem) 32) * 20) 4
+            (mem Ⓓ[4 + mem Ⓓ[ gp ⊖ 920 ⊕ (31 ⊖ clz (uxTopReadyPriority gp mem) 32) * 20 ]]) 4 /\
+        uxTopReadyPriority gp mem = uxTopReadyPriority gp base_mem /\
+        mem Ⓓ[ 4 + mem Ⓓ[ gp ⊖ 920 + (31 ⊖ clz (uxTopReadyPriority gp mem) 32) * 20 ] ] =
+            base_mem Ⓓ[ 4 + base_mem Ⓓ[ gp ⊖ 920 + (31 ⊖ clz (uxTopReadyPriority gp base_mem) 32) * 20 ] ]  /\
+        (uxSchedulerSuspended gp base_mem =? 0) = true /\
         cycle_count_of_trace t' = 9 + 8 * time_mem + time_branch)
-    | 0x800013c4 => Some (exists mem gp, s V_MEM32 = Ⓜmem /\ 
-        s R_GP = Ⓓgp /\ s R_SP = Ⓓ(base_sp ⊖ 16) /\
-        s R_A3 = Ⓓ(mem Ⓓ[4 + mem Ⓓ[48 + pxCurrentTCB gp mem]]) /\
-        s R_A4 = Ⓓ(mem Ⓓ[8 + mem Ⓓ[48 + pxCurrentTCB gp mem]]) /\
-        s R_A5 = Ⓓ(mem Ⓓ[48 + pxCurrentTCB gp mem]) /\
+    | 0x800013c4 => Some (exists mem, s V_MEM32 = Ⓜmem /\ 
+        s R_GP = Ⓓgp /\
         common_noverlaps gp base_sp mem /\
-        (mem Ⓓ[ mem Ⓓ[ 48 + pxCurrentTCB gp mem ] ] =? 0xa5a5a5a5) = true /\
-        (mem Ⓓ[4 + mem Ⓓ[48 + pxCurrentTCB gp mem]] =? mem Ⓓ[mem Ⓓ[48 + pxCurrentTCB gp mem]]) = true /\
-        (uxSchedulerSuspended gp mem =? 0) = true /\
+        mem4_mem4_noverlap_stackframe gp base_sp mem /\
+        mem4_mem4_noverlap_static gp mem /\
+        ~ overlap 32
+            (gp ⊖ 920 ⊕ (31 ⊖ clz (uxTopReadyPriority gp mem) 32) * 20) 4
+            (4 + mem Ⓓ[ gp ⊖ 920 ⊕ (31 ⊖ clz (uxTopReadyPriority gp mem) 32) * 20 ] ) 4 /\
+        ~ overlap 32
+            (gp ⊖ 920 ⊕ (31 ⊖ clz (uxTopReadyPriority gp mem) 32) * 20) 4
+            (mem Ⓓ[4 + mem Ⓓ[ gp ⊖ 920 ⊕ (31 ⊖ clz (uxTopReadyPriority gp mem) 32) * 20 ]]) 4 /\
+        uxTopReadyPriority gp mem = uxTopReadyPriority gp base_mem /\
+        mem Ⓓ[ 4 + mem Ⓓ[ gp ⊖ 920 + (31 ⊖ clz (uxTopReadyPriority gp mem) 32) * 20 ] ] =
+            base_mem Ⓓ[ 4 + base_mem Ⓓ[ gp ⊖ 920 + (31 ⊖ clz (uxTopReadyPriority gp base_mem) 32) * 20 ] ]  /\
+        (uxSchedulerSuspended gp base_mem =? 0) = true /\
         cycle_count_of_trace t' = 12 + 9 * time_mem + time_branch
     )
-    | 0x800013cc => Some (exists mem gp, s V_MEM32 = Ⓜmem /\ 
-        s R_GP = Ⓓgp /\ s R_SP = Ⓓ(base_sp ⊖ 16) /\
-        s R_A3 = Ⓓ(mem Ⓓ[4 + mem Ⓓ[48 + pxCurrentTCB gp mem]]) /\
-        s R_A4 = Ⓓ(mem Ⓓ[8 + mem Ⓓ[48 + pxCurrentTCB gp mem]]) /\
-        s R_A5 = Ⓓ(mem Ⓓ[12 + mem Ⓓ[48 + pxCurrentTCB gp mem]]) /\
+    | 0x800013cc => Some (exists mem, s V_MEM32 = Ⓜmem /\ 
+        s R_GP = Ⓓgp /\
         common_noverlaps gp base_sp mem /\
-        (mem Ⓓ[ mem Ⓓ[ 48 + pxCurrentTCB gp mem ] ] =? 0xa5a5a5a5) = true /\
-        (mem Ⓓ[4 + mem Ⓓ[48 + pxCurrentTCB gp mem]] =? mem Ⓓ[mem Ⓓ[48 + pxCurrentTCB gp mem]]) = true /\
-        (mem Ⓓ[8 + mem Ⓓ[48 + pxCurrentTCB gp mem]] =? mem Ⓓ[4 + mem Ⓓ[48 + pxCurrentTCB gp mem]]) = true /\
-        (uxSchedulerSuspended gp mem =? 0) = true /\
+        mem4_mem4_noverlap_stackframe gp base_sp mem /\
+        mem4_mem4_noverlap_static gp mem /\
+        ~ overlap 32
+            (gp ⊖ 920 ⊕ (31 ⊖ clz (uxTopReadyPriority gp mem) 32) * 20) 4
+            (4 + mem Ⓓ[ gp ⊖ 920 ⊕ (31 ⊖ clz (uxTopReadyPriority gp mem) 32) * 20 ] ) 4 /\
+        ~ overlap 32
+            (gp ⊖ 920 ⊕ (31 ⊖ clz (uxTopReadyPriority gp mem) 32) * 20) 4
+            (mem Ⓓ[4 + mem Ⓓ[ gp ⊖ 920 ⊕ (31 ⊖ clz (uxTopReadyPriority gp mem) 32) * 20 ]]) 4 /\
+        uxTopReadyPriority gp mem = uxTopReadyPriority gp base_mem /\
+        mem Ⓓ[ 4 + mem Ⓓ[ gp ⊖ 920 + (31 ⊖ clz (uxTopReadyPriority gp mem) 32) * 20 ] ] =
+            base_mem Ⓓ[ 4 + base_mem Ⓓ[ gp ⊖ 920 + (31 ⊖ clz (uxTopReadyPriority gp base_mem) 32) * 20 ] ]  /\
+        (uxSchedulerSuspended gp base_mem =? 0) = true /\
         cycle_count_of_trace t' = 15 + 10 * time_mem + time_branch
     )
-    | 0x80001418 => Some (exists mem gp, s V_MEM32 = Ⓜmem /\ 
-        s R_GP = Ⓓgp /\ s R_SP = Ⓓ(base_sp ⊖ 16) /\
+    | 0x80001418 => Some (exists mem, s V_MEM32 = Ⓜmem /\ 
+        s R_GP = Ⓓgp /\
         s R_A1 = Ⓓ(mem Ⓓ[4 + (gp ⊖ 924) ⊕ ((31 ⊖ (clz (uxTopReadyPriority gp mem) 32)) * 20)]) /\
         s R_A2 = Ⓓ(addr_pxReadyTasksLists gp ⊕ ((31 ⊖ (clz (uxTopReadyPriority gp mem) 32)) * 20)) /\
-        s R_A3 = Ⓓ(31 ⊖ clz (uxTopReadyPriority gp mem) 32) /\
-        s R_A4 = Ⓓ(addr_pxReadyTasksLists gp) /\
         s R_A5 = Ⓓ((gp ⊖ 916) ⊕ (31 ⊖ clz (uxTopReadyPriority gp mem) 32) * 20) /\
         common_noverlaps gp base_sp mem /\
-        (uxSchedulerSuspended gp mem =? 0) = true /\
-        cycle_count_of_trace t' = 36 + clz (mem Ⓓ[ 4294965376 + gp ]) 32 + 2 * time_branch + 14 * time_mem)
-    | 0x8000138c => Some (
-        exists mem gp, s V_MEM32 = Ⓜmem /\ s R_GP = Ⓓgp /\ 
-        timing_postcondition t gp mem)
-    | 0x8000144c => Some (
-        exists mem gp, s V_MEM32 = Ⓜmem /\ s R_GP = Ⓓgp /\
-        (* s R_A5 = Ⓓ(mem Ⓓ[12 + mem Ⓓ[48 + pxCurrentTCB gp mem]]) /\ *)
-        timing_postcondition t gp mem)
-    | _ => None end
+        uxTopReadyPriority gp mem = uxTopReadyPriority gp base_mem /\
+        mem Ⓓ[ gp ⊖ 920 + (31 ⊖ clz (uxTopReadyPriority gp mem) 32) * 20 ] =
+            base_mem Ⓓ[ 4 + base_mem Ⓓ[ gp ⊖ 920 + (31 ⊖ clz (uxTopReadyPriority gp base_mem) 32) * 20 ] ]  /\
+        (uxSchedulerSuspended gp base_mem =? 0) = true /\
+        cycle_count_of_trace t' = 36 + clz (uxTopReadyPriority gp mem) 32 + 2 * time_branch + 14 * time_mem)
+    | 0x8000138c | 0x8000144c => Some (time_of_vTaskSwitchContext t gp base_mem)
+    | _ => None
+    end
 | _ => None
 end.
 
+(* The exit points for vTaskSwitchContext *)
+Definition vTaskSwitchContext_exit (t:trace) : bool :=
+  match t with (Addr a,_)::_ => match a with
+  | 0x8000138c | 0x8000144c => true
+  | _ => false
+  end | _ => false end.
+
+(* Lift the code into Picinae IL *)
 Definition lifted_vTaskSwitchContext : program :=
     lift_riscv RTOSDemo_NoAsserts_Clz.
 
+(* Let's build some automation machinery to streamline the proof *)
 Ltac unfold_decompose :=
     cbv [decompose_Btype decompose_Itype decompose_Jtype decompose_Rtype 
         decompose_Stype decompose_Utype mask_bit_section]; cbn [N.land].
 Tactic Notation "unfold_decompose" "in" hyp(H) :=
     cbv [decompose_Btype decompose_Itype decompose_Jtype decompose_Rtype 
         decompose_Stype decompose_Utype mask_bit_section] in H; cbn [N.land] in H.
-
 Ltac unfold_time_of_addr :=
     cbv [time_of_addr neorv32_cycles_upper_bound]; cbn - [setmem getmem].
 Tactic Notation "unfold_time_of_addr" "in" hyp(H) :=
     cbv [time_of_addr neorv32_cycles_upper_bound] in H; cbn - [setmem getmem].
-
 Ltac unfold_cycle_count_list :=
     unfold cycle_count_of_trace; repeat rewrite cycle_count_of_trace_cons, cycle_count_of_trace_single; fold cycle_count_of_trace.
-
 Ltac fold_times :=
     fold time_mem; fold time_branch.
-
 Ltac hammer :=
     unfold_cycle_count_list; unfold_time_of_addr; unfold_decompose; fold_times; psimpl; try lia.
 
+Ltac handle_ex := 
+    repeat (match goal with
+    | [|- exists _, _] => eexists
+    | _ => fail 
+    end); repeat split; try eassumption.
+
+Ltac find_rewrites :=
+    repeat (match goal with
+    | [H: ?x = _ |- context[match ?x with _ => _ end]] =>
+        rewrite H
+    | [H: ?x = _ |- context[if ?x then _ else _]] =>
+        rewrite H
+    | [H: cycle_count_of_trace ?t = _ |- context[cycle_count_of_trace ?t]] =>
+        rewrite H
+    end).
+
+(* We use simpl in a few convenient places: make sure it doesn't go haywire *)
 Arguments N.add _ _ : simpl nomatch.
 Arguments N.mul _ _ : simpl nomatch.
 
-Lemma noverlap_index:
-  forall w a1 len1 a2 len2 index size
-  (NO : ~ overlap w a1 len1 a2 len2)
-  (IN : index + size <= len1),
-  ~ overlap w (a1 + index) size a2 len2.
-Proof.
-  intros.
-  remember (a1 + index) as a1'. apply noverlap_shrink with (a1:=a1) (len1:=len1).
-  rewrite Heqa1'. rewrite add_msub_l.
-  apply N.le_trans with (m:=index+size). rewrite <-N.add_le_mono_r. apply N.Div0.mod_le.
-  assumption.
-  assumption.
-Qed.
-
-Lemma getmem_nbyte_distance:
-  forall w e m a1 a2 n v,
-  msub w a1 a2 > n ->
-  msub w a2 a1 > n ->
-    getmem w e n (setmem w e n m a2 v) a1 = getmem w e n m a1.
-Proof.
-  intros.
-  apply getmem_noverlap.
-  clear - H H0.
-  apply sep_noverlap; try (left; lia || right; lia).
-Qed.
-
-(*
-Define some function f
-- f takes in index into GP 
-- f returns length of buffer that is at mem(gp - index) (or none if malformed)
-Assume in theorem that (forall x y, (assume f x, f y are Some number) 
-    x <> y -> ~ overlap (gp - x) (f x) (gp - y) (f y) )
-Assume (forall x, exists k, f x = Some k -> ~ overlap (gp - x) (f x) (sp (-) 16 16 ))
-Now we can specialize assumption for pxcurrenttcb, uxschedulersuspended etc.
-
-Do we assume that these buffers don't overlap with stack frame?
-*)
-
-Theorem clz_le_w : forall n w,
-    clz n w <= w.
-Proof.
-    destruct n; intros; unfold clz; lia.
-Qed.
+(* The entrypoint to vTaskSwitchContext *)
+Definition start_vTaskSwitchContext : N := 0x8000137c.
 
 Theorem vTaskSwitchContext_timing:
   forall s p t s' x' gp sp mem
-         (ENTRY: startof t (x',s') = (Addr start_vTaskSwitchContext,s)) (* Define the entry point of the function *)
+         (ENTRY: startof t (x',s') = (Addr start_vTaskSwitchContext,s))
          (MDL: models rvtypctx s)
          (GP : s R_GP = Ⓓgp)
          (SP : s R_SP = Ⓓsp)
          (MEM : s V_MEM32 = Ⓜmem)
          (NOVERLAPS : common_noverlaps gp sp mem)
-         (* (GP_SP_FAR : gp_sp_noverlap gp sp)
-         (PCT_NOL_STATIC : pxCurrentTCB_noverlap_static gp mem)
-         (PCT_NOL_SFRAME : pxCurrentTCB_noverlap_stackframe gp sp mem)
-         (MEM_PCT_NOL_SFRAME : mem_pxCurrentTCB_noverlap_stackframe gp sp mem)
-         (MEM_PCT_NOL_STATIC : mem_pxCurrentTCB_noverlap_static gp mem)
-         (SMEM_WELL_FORMED : smem_well_formed gp) *)
+         (MEM4_NOVERLAPS : 
+            mem4_mem4_noverlap_stackframe gp sp mem /\
+            mem4_mem4_noverlap_static gp mem /\
+            ~ overlap 32
+                (gp ⊖ 920 ⊕ (31 ⊖ clz (uxTopReadyPriority gp mem) 32) * 20) 4
+                (4 + mem Ⓓ[ gp ⊖ 920 ⊕ (31 ⊖ clz (uxTopReadyPriority gp mem) 32) * 20 ] ) 4 /\
+            ~ overlap 32
+                (gp ⊖ 920 ⊕ (31 ⊖ clz (uxTopReadyPriority gp mem) 32) * 20) 4
+                (mem Ⓓ[4 + mem Ⓓ[ gp ⊖ 920 ⊕ (31 ⊖ clz (uxTopReadyPriority gp mem) 32) * 20 ]]) 4)
          ,
   satisfies_all 
     lifted_vTaskSwitchContext                                 (* Provide lifted code *)
-    (vTaskSwitchContext_timing_invs s p sp)                  (* Provide invariant set *)
+    (vTaskSwitchContext_timing_invs s p sp gp mem)            (* Provide invariant set *)
     vTaskSwitchContext_exit                                   (* Provide exit point *)
   ((x',s')::t).
 Proof using.
+    (* Set up our proof environment *)
     intros.
     apply prove_invs.
     Local Ltac step := time rv_step.
-    Local Ltac handle_ex := eexists; eexists; repeat split; try eassumption.
-    Local Ltac noverlap_prepare gp sp :=
-        _noverlap_prepare uxSchedulerSuspended pxCurrentTCB 
-            gp_sp_noverlap __global_size vTaskSwitchContext_stack_frame_size 
-            gp sp.
+
+    Local Ltac unfold_vTaskSwitchContext :=
+        unfold uxSchedulerSuspended, __global_size,
+        vTaskSwitchContext_stack_frame_size, uxSchedulerSuspended,
+        gp_sp_noverlap, smem_well_formed, pxCurrentTCB_noverlap_static,
+        pxCurrentTCB_noverlap_stackframe, pxCurrentTCB_noverlap_clz_static,
+        clz_noverlap_smem, mem_pxCurrentTCB_noverlap_stackframe,
+        mem_pxCurrentTCB_noverlap_static, offset_mem_pxCurrentTCB_noverlap_clz,
+        mem4_mem4_noverlap_static, mem4_mem4_noverlap_stackframe,
+        clz_noverlap_sframe, mem4_pxCurrentTCB_noverlap_stackframe,
+        mem4_pxCurrentTCB_noverlap_static, pxCurrentTCB, uxTopReadyPriority,
+        addr_pxReadyTasksLists in *.
+    Local Ltac noverlap_prepare gp sp := 
+        _noverlap_prepare unfold_vTaskSwitchContext gp sp.
     Local Ltac destruct_noverlaps :=
         match goal with
         | [H: common_noverlaps _ _ _ |- _] =>
-            destruct H as [GP_SP_FAR [SMEM_WELL_FORMED [PCT_NOL_STATIC [PCT_NOL_SFRAME [PCT_NOL_CLZ [CLZ_NOL_STATIC [MEM_PCT_NOL_SFRAME MEM_PCT_NOL_STATIC]]]]]]]
-        end.
+            destruct H as [GP_SP_FAR [SMEM_WELL_FORMED [PCT_NOL_STATIC 
+            [PCT_NOL_SFRAME [PCT_NOL_CLZ [CLZ_NOL_STATIC 
+            [MEM_PCT_NOL_SFRAME [MEM_PCT_NOL_STATIC [OFF_MEM_PCT_NOL_CLZ
+            [CLZ_NOL_SFRAME [MEM4_PCT_NOL_SFRAME MEM4_PCT_NOL_STATIC]]]]]]]]]]]
+        end. 
     destruct_noverlaps.
 
     (* Base case *)
     simpl. rewrite ENTRY. step.
-    exists mem, gp. repeat split; try assumption.
-    unfold uxSchedulerSuspended. unfold msub. psimpl. reflexivity.
+    destruct MEM4_NOVERLAPS, H0, H1. unfold uxSchedulerSuspended, msub.
+    handle_ex; now psimpl.
 
     (* Inductive step setup *)
     intros.
     eapply startof_prefix in ENTRY; try eassumption.
     eapply preservation_exec_prog in MDL; 
         try eassumption; [idtac|apply lift_riscv_welltyped].
-    clear - ENTRY PRE MDL. rename t1 into t. rename s1 into s'.
+    clear - ENTRY PRE MDL. rename t1 into t. rename s1 into s'. 
+    rename mem into base_mem.
 
     (* Meat of proof starts here *)
     destruct_inv 32 PRE.
 
     (* 0x800015e4 *)
-    destruct PRE as [mem [gp [MEM [GP [SP [A4 [NOVERLAPS Cycles]]]]]]].
-        destruct_noverlaps.
-    step. step. step. step. step. step. step. step. step. step.
-    do 2 eexists. repeat split. unfold msub. now psimpl.
+    destruct PRE as (mem & MEM & GP & SP & A4 & NOVERLAPS & MEM4_MEM4_NOL_SFRAME
+        & MEM4_MEM4_NOL_STATIC & MEM4_920 & MEM4_MEM4_920 & PreservesPriority
+        & Preserves920 & Cycles). destruct_noverlaps.
+    repeat step. handle_ex.
+        1-10: noverlap_prepare gp sp; memsolve mem gp sp.
+        1-5: noverlap_prepare gp sp; memsolve mem gp sp;
+            try now eapply MEM4_PCT_NOL_STATIC;
+            eauto using noverlap_symmetry.
         {
             noverlap_prepare gp sp.
-            rewrite <- getmem_mod_l with (a := 4294965400 + gp);
-            replace (4294965400 ⊕ gp) with (gp ⊖ 1896) by 
-                (unfold msub; psimpl; lia).
-            memsolve mem gp sp; 
-            try solve [ now (
-                apply PCT_NOL_STATIC ||
-                apply PCT_NOL_SFRAME
-            )].
-            all: apply noverlap_symmetry;
-                (apply noverlap_shrink with (sp ⊖ 16) 16;
-                    [ psimpl; lia | apply noverlap_symmetry]);
-                assumption.
+            repeat rewrite <- getmem_mod_l with (a := _ + _).
+            rewrite getmem_mod_l.
+            replace (clz _ 32) with (clz (uxTopReadyPriority gp mem) 32) by memsolve mem gp sp.
+            replace ((mem [Ⓓgp ⊖ 1932 := 0 ] [Ⓓsp ⊖ 8 := n ] [Ⓓsp ⊖ 4 := n0 ])
+                Ⓓ[ gp ⊖ 920 ⊕ (31 ⊖ clz (uxTopReadyPriority gp mem) 32) * 20 ]) with
+                (mem Ⓓ[ gp ⊖ 920 ⊕ (31 ⊖ clz (uxTopReadyPriority gp mem) 32) * 20 ]); cycle 1.
+                memsolve mem gp sp.
+            rewrite getmem_mod_l.
+            replace ((mem [Ⓓgp ⊖ 1932 := 0 ] [Ⓓsp ⊖ 8 := n ] [Ⓓsp ⊖ 4 := n0 ])
+                Ⓓ[ 4 + mem Ⓓ[ gp ⊖ 920 ⊕ (31 ⊖ clz (uxTopReadyPriority gp mem) 32) * 20 ] ]) with
+                (mem Ⓓ[ 4 + mem Ⓓ[ gp ⊖ 920 ⊕ (31 ⊖ clz (uxTopReadyPriority gp mem) 32) * 20 ] ]); cycle 1.
+                memsolve mem gp sp. now eapply MEM4_PCT_NOL_STATIC.
+            memsolve mem gp sp.
+            unfold uxTopReadyPriority. now repeat rewrite getmem_mod_l; rewrite Preserves920.
+            all: rewrite <- getmem_mod_l. 
+                now eapply MEM4_PCT_NOL_STATIC.
+            all: apply noverlap_shrink with (sp ⊖ 16) 16;
+                [psimpl; lia|auto].
         }
-        {
-            noverlap_prepare gp sp.
-            rewrite <- getmem_mod_l with (a := 4294965400 + gp);
-            replace (4294965400 ⊕ gp) with (gp ⊖ 1896) by 
-                (unfold msub; psimpl; lia).
-            memsolve mem gp sp;
-            try solve [ now (
-                apply PCT_NOL_STATIC ||
-                apply PCT_NOL_SFRAME ||
-                apply MEM_PCT_NOL_STATIC
-            )].
-            all: try solve [apply noverlap_symmetry;
-                (apply noverlap_shrink with (sp ⊖ 16) 16;
-                    [ psimpl; lia | apply noverlap_symmetry]);
-                assumption].
-        } assumption. assumption.
-        {
-            unfold pxCurrentTCB_noverlap_static in *.
-            intros. noverlap_prepare gp sp. memsolve mem gp sp.
-            apply PCT_NOL_STATIC, H.
-        }
-        {
-            unfold pxCurrentTCB_noverlap_stackframe in *.
-            intros. noverlap_prepare gp sp. memsolve mem gp sp.
-            apply PCT_NOL_SFRAME.
-        }
-        {
-            unfold pxCurrentTCB_noverlap_clz_static in *.
-            noverlap_prepare gp sp; memsolve mem gp sp.
-            assumption.
-        }
-        {
-            unfold clz_noverlap_smem in *. intros.
-            noverlap_prepare gp sp; memsolve mem gp sp.
-            eapply CLZ_NOL_STATIC. eassumption.
-        }
-        {
-            unfold mem_pxCurrentTCB_noverlap_stackframe in *.
-            intros. noverlap_prepare gp sp. memsolve mem gp sp.
-                apply MEM_PCT_NOL_SFRAME.
-                now apply PCT_NOL_STATIC.
-                all: apply noverlap_symmetry, noverlap_shrink with (sp ⊖ 16) 16;
-                    [ psimpl; lia |
-                      apply noverlap_symmetry, PCT_NOL_SFRAME ].
-        }
-        {
-            unfold mem_pxCurrentTCB_noverlap_static in *.
-            intros. noverlap_prepare gp sp. memsolve mem gp sp.
-                now apply MEM_PCT_NOL_STATIC.
-                now apply PCT_NOL_STATIC.
-                all: apply noverlap_symmetry, noverlap_shrink with (sp ⊖ 16) 16;
-                    [ psimpl; lia |
-                      apply noverlap_symmetry, PCT_NOL_SFRAME ].
-        }
-        { noverlap_prepare gp sp. memsolve mem gp sp. assumption. }
-        hammer. rewrite A4, BC, Cycles. lia.
-    step. step. handle_ex.
-        unfold timing_postcondition. unfold uxSchedulerSuspended in *.
-            rewrite getmem_frame; try (left; psimpl; lia).
+        hammer. find_rewrites. lia.
+    unfold time_of_vTaskSwitchContext.
         rewrite BC.
-        hammer. rewrite A4, BC, Cycles. lia.
+        hammer. find_rewrites. lia.
 
     (* 0x800013c8 *)
-    destruct PRE as [mem [gp [MEM [GP [SP [A5 [A2 [A4 [NOVERLAPS [BR0 Cycles]]]]]]]]]].
-        destruct_noverlaps.
+    destruct PRE as (mem & MEM & GP & NOVERLAPS & MEM4_MEM4_NOL_SFRAME
+        & MEM4_MEM4_NOL_STATIC & MEM4_920 & MEM4_MEM4_920 & PreservesPriority
+        & Preserves920 & Suspended & Cycles). destruct_noverlaps.
     step.
-        step. step. step. step. step. step. step. step. step. step.
-        exact I. (* Infinite loop, stack overflow detected *)
-    step. handle_ex. change ((678490 << 12) + 1445) with 0xa5a5a5a5 in *.
-        now apply Bool.negb_false_iff in BC.
-        hammer. rewrite A2, A4, BC, Cycles. lia.
-
-    (* 0x800013d0 *)
-    destruct PRE as [mem [gp [MEM [GP [SP [A2 [A3 [A5 [NOVERLAPS [NotSuspended 
-        [Br Cycles]]]]]]]]]]]. destruct_noverlaps.
-    step.
-        step. step. step. step. step. step. step. step. step. step.
+        repeat step.
         exact I. (* Infinite loop, stack overflow detected *)
     step. handle_ex.
-        now apply Bool.negb_false_iff in BC.
-        hammer. rewrite A2, A3, Cycles, BC. lia.
+        hammer. find_rewrites. lia.
+
+    (* 0x800013d0 *)
+    destruct PRE as (mem & MEM & GP & NOVERLAPS & MEM4_MEM4_NOL_SFRAME
+        & MEM4_MEM4_NOL_STATIC & MEM4_920 & MEM4_MEM4_920 & PreservesPriority
+        & Preserves920 & NotSuspended & Cycles). destruct_noverlaps.
+    step.
+        repeat step.
+        exact I. (* Infinite loop, stack overflow detected *)
+    step. handle_ex.
+        hammer. find_rewrites. lia.
 
     (* 0x800013d8 *)
-    destruct PRE as [mem [gp [MEM [GP [SP [A3 [A4 [A5 [NOVERLAPS
-        [B1 [B2 [NotSuspended Cycles]]]]]]]]]]]]. destruct_noverlaps.
+    destruct PRE as (mem & MEM & GP & NOVERLAPS & MEM4_MEM4_NOL_SFRAME
+        & MEM4_MEM4_NOL_STATIC & MEM4_920 & MEM4_MEM4_920 & PreservesPriority
+        & Preserves920 & NotSuspended & Cycles). destruct_noverlaps.
     step.
-        step. step. step. step. step. step. step. step. step. step.
+        repeat step.
         exact I. (* Infinite loop, stack overflow detected *)
-    step.
-        handle_ex.
-        now apply Bool.negb_false_iff in BC.
-        hammer. rewrite A3, A4, BC, Cycles. lia.
+    step. handle_ex.
+        hammer. find_rewrites. lia.
 
     (* 0x800013e0 *)
-    destruct PRE as [mem [gp [MEM [GP [SP [A3 [A4 [A5 [NOVERLAPS [B1 [B2 [B3 
-        [NotSuspended Cycles]]]]]]]]]]]]]. destruct_noverlaps.
-    step. step. step. step. step. step. step. step. step. step. step.
-    step. step. step. step.
-        handle_ex. repeat split.
+    destruct PRE as (mem & MEM & GP & NOVERLAPS & MEM4_MEM4_NOL_SFRAME
+        & MEM4_MEM4_NOL_STATIC & MEM4_920 & MEM4_MEM4_920 & PreservesPriority
+        & Preserves920 & NotSuspended & Cycles). destruct_noverlaps.
+    repeat step.
+        handle_ex.
+        par: try solve [noverlap_prepare gp sp; memsolve mem gp sp].
         {
-            unfold uxTopReadyPriority.
             noverlap_prepare gp sp.
-            rewrite <- getmem_mod_l with (a := 4294965376 + gp);
-            replace (4294965376 ⊕ gp) with (gp ⊖ 1920) by 
-                (unfold msub; psimpl; lia).
-            rewrite <- getmem_mod_l with (a := 4294966376 + gp + 
-                (31 ⊖ clz (mem Ⓓ[ gp ⊖ 1920 ]) 32) * 20).
-            replace (mem Ⓓ[ 4294966376 + gp ⊕ (31 ⊖ clz (mem Ⓓ[ gp ⊖ 1920 ]) 32) * 20 ])
-            with (mem Ⓓ[ gp ⊖ 920 ⊕ (31 ⊖ clz (mem Ⓓ[ gp ⊖ 1920 ]) 32) * 20 ]); cycle 7.
-                unfold msub at 1; now psimpl.
-            rewrite <- setmem_mod_l, (N.add_comm 4294966376).
-            assert (forall n, gp + 4294966376 ⊕ n = gp ⊖ 920 ⊕ n). {
-                intros. unfold msub. simpl (_ - _ mod _).
-                now psimpl.
-            } rewrite H. clear H.
-            assert (forall n, 4 + (gp ⊖ 924) ⊕ n = (gp ⊖ 920) ⊕ n).
-                intros; unfold msub; simpl (_ - _ mod _); now psimpl.
-            rewrite H. clear H. psimpl.
             replace (clz
             ((mem [Ⓓgp ⊖ 920 ⊕ (31 ⊖ clz (mem Ⓓ[ gp ⊖ 1920 ]) 32) * 20
               := mem
-                 Ⓓ[ 4 + mem Ⓓ[ gp ⊖ 920 ⊕ (31 ⊖ clz (mem Ⓓ[ gp ⊖ 1920 ]) 32) * 20 ]
-                 ] ]) Ⓓ[ gp ⊖ 1920 ]) 32) with 
-                (clz (mem Ⓓ[ gp ⊖ 1920 ]) 32); cycle 1. {
-                f_equal. memsolve mem gp sp.
-                apply sep_noverlap; left; psimpl;
-                pose proof (clz_le_w (mem Ⓓ[ gp ⊖ 1920 ]) 32);
-                remember (clz (mem Ⓓ[ gp ⊖ 1920 ]) 32) as n; clear Heqn;
-                do 33 (destruct n as [| n _] using N.peano_ind;
-                    [cbn [N.succ Pos.succ]; psimpl; lia|
-                    replace (N.succ n) with (1 + n) in H by lia; psimpl in H]);
-                lia.
-            } psimpl. reflexivity.
-        }
-        {
-            unfold addr_pxReadyTasksLists, uxTopReadyPriority.
-            noverlap_prepare gp sp; memsolve mem gp sp. f_equal.
-                unfold msub; psimpl.
-                replace (2 ^ 32 - 1920 mod 2 ^ 32) with 4294965376 by reflexivity.
-                now rewrite getmem_mod_l, (N.add_comm gp).
-            unfold msub at 1; psimpl.
-            apply sep_noverlap; left; psimpl;
-                pose proof (clz_le_w (mem Ⓓ[ 4294965376 + gp ]) 32);
-                remember (clz (mem Ⓓ[ 4294965376 + gp ]) 32) as n; clear Heqn;
-                do 33 (destruct n as [| n _] using N.peano_ind;
-                    [cbn [N.succ Pos.succ]; psimpl; lia|
-                    replace (N.succ n) with (1 + n) in H by lia; psimpl in H]);
-                lia.
-        }
-        {
-            unfold uxTopReadyPriority.
+                 Ⓓ[ 4 +
+                    mem Ⓓ[ gp ⊖ 920 ⊕ (31 ⊖ clz (mem Ⓓ[ gp ⊖ 1920 ]) 32) * 20
+                    ] ] ]) Ⓓ[ gp ⊖ 1920 ]) 32) with 
+                (clz (mem Ⓓ[ gp ⊖ 1920 ]) 32) by
+                (f_equal; memsolve mem gp sp; auto).
+            unfold msub. now psimpl.
+        } {
             noverlap_prepare gp sp; memsolve mem gp sp.
-                unfold msub at 3. simpl (_ - _ mod _).
-                now rewrite getmem_mod_l, (N.add_comm 4294965376).
-            apply sep_noverlap; left; psimpl;
-                pose proof (clz_le_w (mem Ⓓ[ 4294965376 + gp ]) 32);
-                remember (clz (mem Ⓓ[ 4294965376 + gp ]) 32) as n; clear Heqn;
-                do 33 (destruct n as [| n _] using N.peano_ind;
-                    [cbn [N.succ Pos.succ]; psimpl; lia|
-                    replace (N.succ n) with (1 + n) in H by lia; psimpl in H]);
-                lia.
-        }
-        now unfold addr_pxReadyTasksLists, msub; psimpl.
-        {
-            unfold uxTopReadyPriority.
-            noverlap_prepare gp sp; memsolve mem gp sp. f_equal.
-                unfold msub at 2 4. simpl (_ - _ mod _).
-                rewrite N.add_comm, N.add_assoc.
-                rewrite (N.add_comm _ gp), getmem_mod_l. now psimpl.
-            apply sep_noverlap; left; psimpl;
-                pose proof (clz_le_w (mem Ⓓ[ 4294965376 + gp ]) 32);
-                remember (clz (mem Ⓓ[ 4294965376 + gp ]) 32) as n; clear Heqn;
-                do 33 (destruct n as [| n _] using N.peano_ind;
-                    [cbn [N.succ Pos.succ]; psimpl; lia|
-                    replace (N.succ n) with (1 + n) in H by lia; psimpl in H]);
-                lia.
-        }
-        {
-            unfold pxCurrentTCB_noverlap_static. intros.
-            noverlap_prepare gp sp; memsolve mem gp sp.
-            now apply PCT_NOL_STATIC.
-            unfold msub at 1. simpl (_ - _ mod _).
-            apply sep_noverlap; left; psimpl;
-                pose proof (clz_le_w (mem Ⓓ[ 4294965376 + gp ]) 32);
-                remember (clz (mem Ⓓ[ 4294965376 + gp ]) 32) as n; clear Heqn;
-                do 33 (destruct n as [| n _] using N.peano_ind;
-                    [cbn [N.succ Pos.succ]; psimpl; lia|
-                    replace (N.succ n) with (1 + n) in H by lia; psimpl in H]);
-                lia.
-        }
-        {
-            unfold pxCurrentTCB_noverlap_stackframe. intros.
-            noverlap_prepare gp sp; memsolve mem gp sp.
-            now apply PCT_NOL_SFRAME.
-            unfold msub at 1. simpl (_ - _ mod _).
-            apply sep_noverlap; left; psimpl;
-                pose proof (clz_le_w (mem Ⓓ[ 4294965376 + gp ]) 32);
-                remember (clz (mem Ⓓ[ 4294965376 + gp ]) 32) as n; clear Heqn;
-                do 33 (destruct n as [| n _] using N.peano_ind;
-                    [cbn [N.succ Pos.succ]; psimpl; lia|
-                    replace (N.succ n) with (1 + n) in H by lia; psimpl in H]);
-                lia.
-        }
-        {
-            unfold pxCurrentTCB_noverlap_clz_static.
-            noverlap_prepare gp sp; memsolve mem gp sp.
-            now apply PCT_NOL_CLZ.
-            all: unfold msub at 1; simpl (_ - _ mod _);
-            apply sep_noverlap; left; psimpl;
-                pose proof (clz_le_w (mem Ⓓ[ 4294965376 + gp ]) 32);
-                remember (clz (mem Ⓓ[ 4294965376 + gp ]) 32) as n; clear Heqn;
-                do 33 (destruct n as [| n _] using N.peano_ind;
-                    [cbn [N.succ Pos.succ]; psimpl; lia|
-                    replace (N.succ n) with (1 + n) in H by lia; psimpl in H]);
-                lia.
-        }
-        {
-            unfold clz_noverlap_smem in *. intros.
-            replace ((mem
-            [Ⓓ4294966376 + gp + (31 ⊖ clz (mem Ⓓ[ 4294965376 + gp ]) 32) * 20
+            unfold msub. psimpl.
+            now rewrite N.add_comm, N.add_assoc,
+                (N.add_comm _ gp), getmem_mod_l.
+        } {
+            noverlap_prepare gp sp.
+            replace ((mem [Ⓓgp ⊖ 920 ⊕ (31 ⊖ clz (mem Ⓓ[ gp ⊖ 1920 ]) 32) * 20
             := mem
                Ⓓ[ 4 +
-                  mem
-                  Ⓓ[ 4294966376 + gp +
-                     (31 ⊖ clz (mem Ⓓ[ 4294965376 + gp ]) 32) * 20 ] ] ])
-           Ⓓ[ gp ⊖ 1920 ]) with (mem Ⓓ[gp ⊖ 1920]).
-           eapply CLZ_NOL_STATIC. eassumption.
-           rewrite <- setmem_mod_l.
-           rewrite <- getmem_mod_l with (a := 4294966376 + gp + (31 ⊖ clz (mem Ⓓ[ 4294965376 + gp ]) 32) * 20).
-           rewrite getmem_noverlap. reflexivity.
-           rewrite <- getmem_mod_l. 
-           replace (mem Ⓓ[ 4294965376 ⊕ gp ]) with (mem Ⓓ[ gp ⊖ 1920 ]) by (unfold msub; psimpl; lia).
-           replace (4294966376 + gp ⊕ (31 ⊖ clz (mem Ⓓ[ gp ⊖ 1920 ]) 32) * 20) with
-                (gp ⊖ 920 ⊕ (31 ⊖ clz (mem Ⓓ[ gp ⊖ 1920 ]) 32) * 20).
-           now eapply CLZ_NOL_STATIC.
-           now unfold msub at 1; psimpl.
-        }
-        {
-            unfold mem_pxCurrentTCB_noverlap_stackframe.
-            replace (mem Ⓓ[ 4294966376 + gp + (31 ⊖ clz (mem Ⓓ[ 4294965376 + gp ]) 32) * 20 ])
-                with (mem Ⓓ[ (gp ⊖ 920) + (31 ⊖ clz (mem Ⓓ[ gp ⊖ 1920 ]) 32) * 20 ]).
-            replace (mem [Ⓓ4294966376 + gp + (31 ⊖ clz (mem Ⓓ[ 4294965376 + gp ]) 32) * 20
-                := mem Ⓓ[ 4 + mem Ⓓ[ gp ⊖ 920 + (31 ⊖ clz (mem Ⓓ[ gp ⊖ 1920 ]) 32) * 20 ]]])
-                with (mem [Ⓓ(gp ⊖ 920) + (31 ⊖ clz (mem Ⓓ[ 4294965376 + gp ]) 32) * 20
-                := mem Ⓓ[ 4 + mem Ⓓ[ gp ⊖ 920 + (31 ⊖ clz (mem Ⓓ[ gp ⊖ 1920 ]) 32) * 20 ]]]).
-            rewrite <- setmem_mod_l.
-            noverlap_prepare gp sp; memsolve mem gp sp.
-            now apply MEM_PCT_NOL_SFRAME.
-            all: try solve [unfold msub at 1; simpl (_ - _ mod _);
-                apply sep_noverlap; left; psimpl;
-                pose proof (clz_le_w (mem Ⓓ[ 4294965376 + gp ]) 32);
-                remember (clz (mem Ⓓ[ 4294965376 + gp ]) 32) as n; clear Heqn;
-                do 33 (destruct n as [| n _] using N.peano_ind;
-                    [cbn [N.succ Pos.succ]; psimpl; lia|
-                    replace (N.succ n) with (1 + n) in H by lia; psimpl in H]);
-                lia].
-            replace (mem Ⓓ[ 4294965376 + gp ]) with (mem Ⓓ[gp ⊖ 1920]) by 
-                (unfold msub; simpl (_ - _ mod _); psimpl; lia).
-            apply PCT_NOL_CLZ.
-            unfold msub at 1. simpl (_ - _ mod _).
-                rewrite <- setmem_mod_l with 
-                    (a := gp ⊕ 4294966376 + (31 ⊖ clz (mem Ⓓ[ 4294965376 + gp ]) 32) * 20).
-                rewrite <- setmem_mod_l with
-                    (a := 4294966376 + gp + (31 ⊖ clz (mem Ⓓ[ 4294965376 + gp ]) 32) * 20).
-                now psimpl.
-            unfold msub at 1 3; simpl (_ - _ mod _).
-                rewrite getmem_mod_l; psimpl.
-                now rewrite (N.add_comm gp).
-        }
-        {
-            unfold mem_pxCurrentTCB_noverlap_static. intros.
+                  mem Ⓓ[ gp ⊖ 920 ⊕ (31 ⊖ clz (mem Ⓓ[ gp ⊖ 1920 ]) 32) * 20 ]
+               ] ]) Ⓓ[ gp ⊖ 1920 ]) with (mem Ⓓ[ gp ⊖ 1920 ]) by
+               (rewrite getmem_noverlap; auto). psimpl.
+            rewrite <- getmem_mod_l with (a := _ ⊖ _ + _). eauto.
+        } {
             noverlap_prepare gp sp.
-            rewrite <- getmem_mod_l with (a := 4294965376 + gp);
-            replace (4294965376 ⊕ gp) with (gp ⊖ 1920) by 
-                (unfold msub; psimpl; lia).
-            rewrite <- getmem_mod_l with (a := 4294966376 + gp + 
-                (31 ⊖ clz (mem Ⓓ[ gp ⊖ 1920 ]) 32) * 20).
-            replace (mem Ⓓ[ 4294966376 + gp ⊕ (31 ⊖ clz (mem Ⓓ[ gp ⊖ 1920 ]) 32) * 20 ])
-            with (mem Ⓓ[ gp ⊖ 920 ⊕ (31 ⊖ clz (mem Ⓓ[ gp ⊖ 1920 ]) 32) * 20 ]); cycle 7.
-                unfold msub at 1; now psimpl.
-            rewrite <- setmem_mod_l, (N.add_comm 4294966376).
-            assert (forall n, gp + 4294966376 ⊕ n = gp ⊖ 920 ⊕ n).
-                intros; unfold msub; simpl (_ - _ mod _);
-                now psimpl.
-            rewrite H0. clear H0. psimpl.
-            replace ((mem [Ⓓgp ⊖ 920 + (31 ⊖ clz (mem Ⓓ[ gp ⊖ 1920 ]) 32) * 20
-                := mem Ⓓ[ 4 + mem Ⓓ[ gp ⊖ 920 + (31 ⊖ clz (mem Ⓓ[ gp ⊖ 1920 ]) 32) * 20 ] ] ])
-            Ⓓ[ 48 +
-                (mem [Ⓓgp ⊖ 920 + (31 ⊖ clz (mem Ⓓ[ gp ⊖ 1920 ]) 32) * 20
-                := mem Ⓓ[ 4 + mem Ⓓ[ gp ⊖ 920 + (31 ⊖ clz (mem Ⓓ[ gp ⊖ 1920 ]) 32) * 20 ] ] ])
-                Ⓓ[ gp ⊖ 1896 ] ]) with (mem Ⓓ[48 + pxCurrentTCB gp mem]).
-            now apply MEM_PCT_NOL_STATIC.
-            rewrite <- setmem_mod_l with (a := gp ⊖ 920 + (31 ⊖ clz (mem Ⓓ[ gp ⊖ 1920 ]) 32) * 20).
-            memsolve mem gp sp. reflexivity.
-            (* unfold msub at 1 4; simpl (_ - _ mod _). *)
-            all: try solve [unfold msub at 1 4; simpl (_ - _ mod _);
-                apply sep_noverlap; left; psimpl;
-                pose proof (clz_le_w (mem Ⓓ[ gp ⊕ 4294965376 ]) 32);
-                remember (clz (mem Ⓓ[ gp ⊕ 4294965376 ]) 32) as n; clear Heqn;
-                do 33 (destruct n as [| n _] using N.peano_ind;
-                    [cbn [N.succ Pos.succ]; psimpl; lia|
-                    replace (N.succ n) with (1 + n) in H by lia; psimpl in H]);
-                lia].
-            assumption.
+            replace (clz ((mem [Ⓓ_ := _ ]) Ⓓ[ gp ⊖ 1920 ]) 32) 
+                with (clz (mem Ⓓ[ gp ⊖ 1920 ]) 32) by
+                (f_equal; rewrite getmem_noverlap; auto).
+            psimpl.
+            rewrite <- getmem_mod_l with (a := gp ⊖ _ + _).
+            eauto.
+        } { 
+            noverlap_prepare gp sp.
+            replace (clz ((mem [Ⓓ_ := _ ]) Ⓓ[ gp ⊖ 1920 ]) 32) 
+                with (clz (mem Ⓓ[ gp ⊖ 1920 ]) 32) by
+                (f_equal; rewrite getmem_noverlap; auto).
+            psimpl. auto.
         }
-        {
-            noverlap_prepare gp sp; memsolve mem gp sp.
-            assumption.
-            apply sep_noverlap; left; psimpl;
-                pose proof (clz_le_w (mem Ⓓ[ 4294965376 + gp ]) 32);
-                remember (clz (mem Ⓓ[ 4294965376 + gp ]) 32) as n; clear Heqn;
-                do 33 (destruct n as [| n _] using N.peano_ind;
-                    [cbn [N.succ Pos.succ]; psimpl; lia|
-                    replace (N.succ n) with (1 + n) in H by lia; psimpl in H]);
-                lia.
-        }
-        hammer. rewrite A4, A5, BC, Cycles. psimpl.
-        (* Can't infer placeholder? *)
-        replace ((mem[Ⓓ4294966376 + gp + (31 ⊖ clz (mem Ⓓ[ 4294965376 + gp ]) 32) * 20
-                    := mem Ⓓ[ 4 + mem Ⓓ[ 4294966376 + gp + 
-                                (31 ⊖ clz (mem Ⓓ[ 4294965376 + gp ]) 32) * 20 ]
-                            ] 
-                    ]) Ⓓ[ 4294965376 + gp ]) with (mem Ⓓ[ 4294965376 + gp ]).
+        hammer. find_rewrites. psimpl.
+        noverlap_prepare gp sp.
+        replace (clz ((mem [Ⓓ_ := _ ]) Ⓓ[ gp ⊖ 1920 ]) 32) 
+                with (clz (mem Ⓓ[ gp ⊖ 1920 ]) 32) by
+                (f_equal; rewrite getmem_noverlap; auto).
         lia.
-        {
-            noverlap_prepare gp sp. memsolve mem gp sp.
-            apply sep_noverlap; left; psimpl;
-                pose proof (clz_le_w (mem Ⓓ[ 4294965376 + gp ]) 32);
-                remember (clz (mem Ⓓ[ 4294965376 + gp ]) 32) as n; clear Heqn;
-                do 33 (destruct n as [| n _] using N.peano_ind;
-                    [cbn [N.succ Pos.succ]; psimpl; lia|
-                    replace (N.succ n) with (1 + n) in H by lia; psimpl in H]);
-                lia.
-        }
-    (* Inside vApplicationStackOverflowHook *)
-    step. step. step. step. step. step. step. step. step. step. exact I.
 
-    (* 0x8000142c *)
-    destruct PRE as [mem [gp [MEM [GP [SP [A1 [A2 [A3 [A4 [A5 [NOVERLAPS 
-        [NotSuspended Cycles]]]]]]]]]]]]. destruct_noverlaps.
-    step. step. step. step. step. step. step. step. step. step. step.
-        handle_ex. unfold timing_postcondition.
-        replace (uxSchedulerSuspended gp _ =? 0) with true.
-        apply Bool.negb_true_iff in BC.
-        hammer. rewrite A1, A5, BC, Cycles.
-        cbn [negb]. replace (_ =? _) with 
-        (mem Ⓓ[ 4 + (gp ⊖ 924) ⊕ (31 ⊖ clz (uxTopReadyPriority gp mem) 32) * 20 ] =?
-            gp ⊖ 916 ⊕ (31 ⊖ clz (uxTopReadyPriority gp mem) 32) * 20).
-        rewrite BC. replace (
-            clz ((mem [Ⓓ4294965400 + gp := 
-                mem Ⓓ[ 12 + mem Ⓓ[ 4 + addr_pxReadyTasksLists gp +
-                        (31 ⊖ clz (uxTopReadyPriority gp mem) 32) * 20 ] ] ])
-                Ⓓ[ 4294965376 + gp ]) 32) with 
-            (clz (mem Ⓓ[ 4294965376 + gp ]) 32).
-        lia.
-        noverlap_prepare gp n; memsolve mem gp n.
-        { unfold addr_pxReadyTasksLists, uxTopReadyPriority.
-          noverlap_prepare gp n.
-          rewrite <- getmem_mod_l with (
-            a := gp ⊖ 920 +
-            (31
-             ⊖ clz
-                 ((mem [Ⓓgp ⊖ 1896
-                   := mem
-                      Ⓓ[ 12 + mem Ⓓ[ 4 + (gp ⊖ 924) + (31 ⊖ clz (mem Ⓓ[ gp ⊖ 1920 ]) 32) * 20 ] ]
-                   ]) Ⓓ[ gp ⊖ 1920 ]) 32) * 20
-          ). memsolve mem gp n.
-          now apply noverlap_symmetry, CLZ_NOL_STATIC.
-        }
-        { unfold uxSchedulerSuspended. noverlap_prepare gp n. memsolve mem gp n.
-          now rewrite NotSuspended. }
-    step. step. step. step. step. step. step. step. step. step. step.
-    step.
-        handle_ex.
-        unfold timing_postcondition.
-        replace (uxSchedulerSuspended gp _ =? 0) with true.
-        apply Bool.negb_false_iff in BC.
-        hammer. rewrite A1, A5, BC, Cycles.
-        match goal with
-        | [H: (?a =? ?b) = true |- _ = (if ?x =? ?y then _ else _) ] =>
-            replace (x =? y) with (a =? b); [rewrite H|idtac]
-        | _ => idtac end.
-        cbn [negb].
-        replace (clz
-        ((mem [Ⓓ4 + addr_pxReadyTasksLists gp + (31 ⊖ clz (uxTopReadyPriority gp mem) 32) * 20
-          := mem
-             Ⓓ[ 12 + addr_pxReadyTasksLists gp + (31 ⊖ clz (uxTopReadyPriority gp mem) 32) * 20
-             ] ] [Ⓓ4294965400 + gp
-          := (mem
-              [Ⓓ4 + addr_pxReadyTasksLists gp + (31 ⊖ clz (uxTopReadyPriority gp mem) 32) * 20
-              := mem
-                 Ⓓ[ 12 + addr_pxReadyTasksLists gp +
-                    (31 ⊖ clz (uxTopReadyPriority gp mem) 32) * 20 ] ])
-             Ⓓ[ 12 +
-                mem
-                Ⓓ[ 12 + addr_pxReadyTasksLists gp +
-                   (31 ⊖ clz (uxTopReadyPriority gp mem) 32) * 20 ] ] ]) Ⓓ[ 
-         4294965376 + gp ]) 32) 
-        with (clz (mem Ⓓ[ 4294965376 + gp ]) 32).
-        lia.
-        { f_equal.
-            unfold addr_pxReadyTasksLists, uxTopReadyPriority.
-            noverlap_prepare gp sp; memsolve mem gp sp.
-            unfold msub at 1 3; simpl (_ - _ mod _).
-            apply sep_noverlap; left; psimpl;
-                pose proof (clz_le_w (mem Ⓓ[ gp ⊕ 4294965376 ]) 32);
-                remember (clz (mem Ⓓ[ gp ⊕ 4294965376 ]) 32) as n; clear Heqn;
-                do 33 (destruct n as [| n _] using N.peano_ind;
-                    [cbn [N.succ Pos.succ]; psimpl; lia|
-                    replace (N.succ n) with (1 + n) in H by lia; psimpl in H]);
-                lia.
-        }
-        {
-            (* unfold addr_pxReadyTasksLists, uxTopReadyPriority.
-            noverlap_prepare gp sp.
-            match goal with
-            | [|- context[?M [Ⓓ?X + ?Y := _]]] =>
-                rewrite <- setmem_mod_l with (a := X + Y)
-            end.
-            memsolve mem gp sp.
-            all: try solve [unfold msub at 1 4; simpl (_ - _ mod _);
-                apply sep_noverlap; left; psimpl;
-                    pose proof (clz_le_w (mem Ⓓ[ gp ⊕ 4294965376 ]) 32);
-                    remember (clz (mem Ⓓ[ gp ⊕ 4294965376 ]) 32) as n; clear Heqn;
-                    do 33 (destruct n as [| n _] using N.peano_ind;
-                        [cbn [N.succ Pos.succ]; psimpl; lia|
-                        replace (N.succ n) with (1 + n) in H by lia; psimpl in H]);
-                    lia].
-            2: try solve [apply noverlap_symmetry; unfold msub at 1 4; 
-                simpl (_ - _ mod _); apply sep_noverlap; left; psimpl;
-                pose proof (clz_le_w (mem Ⓓ[ gp ⊕ 4294965376 ]) 32);
-                remember (clz (mem Ⓓ[ gp ⊕ 4294965376 ]) 32) as n; clear Heqn;
-                do 33 (destruct n as [| n _] using N.peano_ind;
-                    [cbn [N.succ Pos.succ]; psimpl; lia|
-                    replace (N.succ n) with (1 + n) in H by lia; psimpl in H]);
-                lia]. *)
-            admit. (* Overlapping *)
-        }
-        { unfold addr_pxReadyTasksLists, uxTopReadyPriority; 
-            noverlap_prepare gp n0; memsolve mem gp n0. now rewrite NotSuspended.
-            unfold msub at 1 4; 
-                simpl (_ - _ mod _); apply sep_noverlap; left; psimpl;
-                pose proof (clz_le_w (mem Ⓓ[ gp ⊕ 4294965376 ]) 32);
-                remember (clz (mem Ⓓ[ gp ⊕ 4294965376 ]) 32) as n; clear Heqn;
-                do 33 (destruct n as [| n _] using N.peano_ind;
-                    [cbn [N.succ Pos.succ]; psimpl; lia|
-                    replace (N.succ n) with (1 + n) in H by lia; psimpl in H]);
-                lia. }
-    step. exact I.
-Admitted.
+    destruct PRE as (mem & MEM & GP & A1 & A2 & A5 & NOVERLAPS
+        & PreservesPriority & Preserves920 & NotSuspended & Cycles).
+    destruct_noverlaps.
+    repeat step.
+    unfold time_of_vTaskSwitchContext.
+        find_rewrites.
+        hammer. rewrite <- Preserves920, <- PreservesPriority.
+        find_rewrites.
+        replace (4 + (gp ⊖ 924) ⊕ (31 ⊖ clz (uxTopReadyPriority gp mem) 32) * 20) with
+            ((gp ⊖ 920) ⊕ (31 ⊖ clz (uxTopReadyPriority gp mem) 32) * 20) in BC by
+            (unfold msub; now psimpl).
+        rewrite Bool.negb_true_iff, getmem_mod_l in BC.
+        find_rewrites. lia.
+    unfold time_of_vTaskSwitchContext.
+        find_rewrites. hammer. find_rewrites.
+        rewrite <- Preserves920, <- PreservesPriority.
+        replace (4 + _ ⊕ _) with ((gp ⊖ 920) ⊕ (31 ⊖ clz (mem Ⓓ[ gp ⊖ 1920 ]) 32) * 20)
+            in BC by (unfold msub; now psimpl).
+        unfold uxTopReadyPriority in *.
+        rewrite Bool.negb_false_iff, getmem_mod_l in BC.
+        find_rewrites. lia.
+
+    now repeat step.
+Qed.
